add unfolding lemmas

src/FIFOSched.v
@@ -1,4 +1,6 @@
+From sflib Require Import sflib.
 Require Import Program.
+From ExtLib Require Import FMapAList.
 From Fairness Require Import
   Mod
   Concurrency.
@@ -38,20 +40,101 @@ Section SCHEDULE.
         exact (Vis (inr1 e) (fun x => Ret (inl (tid, k x)))).
   Defined.
   
+  Definition pick_thread_fifo {R} :
+    tids.(id) * (itree Es R + R) ->
+    alist tids.(id) (itree Es R) ->
+    itree (eventE2 +' E) (tids.(id) * itree Es R * alist tids.(id) (itree Es R) + R) :=
+    fun '(tid, res) ts =>
+      match res with
+      | inl t => match (ts ++ [(tid, t)]) with
+                | [] => Vis (inl1 (Choose void)) (Empty_set_rect _)
+                | t' :: ts' => Ret (inl (t', ts'))
+                end
+      | inr r => match ts with
+                | [] => Ret (inr r)
+                | t' :: ts' => Ret (inl (t', ts'))
+                end
+      end.
+
   Definition interp_fifosched {R} :
-    @threads _ E R -> itree (eventE2 +' E) ().
+    tids.(id) * itree Es R * alist tids.(id) (itree Es R) -> itree (eventE2 +' E) R :=
+    ITree.iter (fun '(t,ts) =>
+                  res <- interp_thread_nonpreemtive t;;
+                  pick_thread_fifo (fst t, res) ts
+      ).
+
+  Lemma unfold_interp_fifosched {R} tid (t : itree Es R) ts :
+    interp_fifosched (tid, t, ts) =
+      res <- interp_thread_nonpreemtive (tid, t);;
+      yr <- pick_thread_fifo (tid, res) ts;;
+      match yr with
+      | inl y => tau;; interp_fifosched y
+      | inr r => Ret r
+      end.
   Proof.
-    eapply ITree.iter.
-    intros [| [tid t] ts].
-    - (* No thread to execute *)
-      exact (Ret (inr tt)).
-    - eapply ITree.bind.
-      + eapply (interp_thread_nonpreemtive (tid, t)).
-      + intros [t' | r].
-        * (* thread t yielded *)
-          exact (Ret (inl (ts ++ [(tid, t')]))).
-        * (* thread t terminated with r *)
-          exact (Ret (inl ts)).
-  Defined.
+    unfold interp_fifosched at 1, curry.
+    rewrite unfold_iter at 1. rewrite bind_bind.
+    reflexivity.
+  Qed.
+
+  Lemma interp_thread_nonpreemtive_ret {R} tid (r : R) :
+    interp_thread_nonpreemtive (tid, Ret r) = Ret (inr r).
+  Proof. unfold interp_thread_nonpreemtive. rewrite unfold_iter. ss. rewrite bind_ret_l. ss. Qed.
+
+  Lemma interp_thread_nonpreemtive_tau R tid (itr : itree Es R) :
+    interp_thread_nonpreemtive (tid, tau;; itr) = tau;; interp_thread_nonpreemtive (tid, itr).
+  Proof. unfold interp_thread_nonpreemtive at 1. rewrite unfold_iter. ss. rewrite bind_ret_l. ss. Qed.
+
+  Lemma interp_thread_nonpreemtive_vis R tid X (e : E X) (ktr : ktree Es X R) :
+    interp_thread_nonpreemtive (tid, Vis (inr1 e) ktr) =
+      Vis (inr1 e) (fun x => tau;; interp_thread_nonpreemtive (tid, ktr x)).
+  Proof.
+    unfold interp_thread_nonpreemtive at 1. rewrite unfold_iter. ss. rewrite bind_vis.
+    eapply (f_equal (fun x => Vis (inr1 e) x)). extensionality x.
+    rewrite bind_ret_l. ss.
+  Qed.
+
+  Lemma interp_thread_nonpreemtive_trigger R tid X (e : E X) (ktr : ktree Es X R) :
+    interp_thread_nonpreemtive (tid, x <- trigger (inr1 e);; ktr x) =
+      x <- trigger (inr1 e);; tau;; interp_thread_nonpreemtive (tid, ktr x).
+  Proof. rewrite ! bind_trigger. eapply interp_thread_nonpreemtive_vis. Qed.
+
+  Lemma interp_thread_nonpreemtive_vis_eventE R tid X (e : eventE2 X) (ktr : ktree Es X R) :
+    interp_thread_nonpreemtive (tid, Vis (inl1 (inl1 e)) ktr) =
+      Vis (inl1 e) (fun x => tau;; interp_thread_nonpreemtive (tid, ktr x)).
+  Proof.
+    unfold interp_thread_nonpreemtive at 1. rewrite unfold_iter. ss. rewrite bind_vis.
+    eapply (f_equal (fun x => Vis (inl1 e) x)). extensionality x.
+    rewrite bind_ret_l. ss.
+  Qed.
+
+  Lemma interp_thread_nonpreemtive_trigger_eventE R tid X (e : eventE2 X) (ktr : ktree Es X R) :
+    interp_thread_nonpreemtive (tid, x <- trigger (inl1 (inl1 e));; ktr x) =
+      x <- trigger (inl1 e);; tau;; interp_thread_nonpreemtive (tid, ktr x).
+  Proof. rewrite ! bind_trigger. eapply interp_thread_nonpreemtive_vis_eventE. Qed.
+
+  Lemma interp_thread_nonpreemtive_vis_gettid R tid (ktr : ktree Es tids.(id) R) :
+    interp_thread_nonpreemtive (tid, Vis (inl1 (inr1 GetTid)) ktr) =
+      tau;; interp_thread_nonpreemtive (tid, ktr tid).
+  Proof.
+    unfold interp_thread_nonpreemtive at 1. rewrite unfold_iter. ss. rewrite bind_ret_l. ss.
+  Qed.
+
+  Lemma interp_thread_nonpreemtive_trigger_gettid R tid (ktr : ktree Es tids.(id) R) :
+    interp_thread_nonpreemtive (tid, x <- trigger (inl1 (inr1 GetTid));; ktr x) =
+      tau;; interp_thread_nonpreemtive (tid, ktr tid).
+  Proof. rewrite bind_trigger. eapply interp_thread_nonpreemtive_vis_gettid. Qed.
+
+  Lemma interp_thread_nonpreemtive_vis_yield R tid (ktr : ktree Es () R) :
+    interp_thread_nonpreemtive (tid, Vis (inl1 (inr1 Yield)) ktr) =
+      Ret (inl (ktr tt)).
+  Proof.
+    unfold interp_thread_nonpreemtive at 1. rewrite unfold_iter. ss. rewrite bind_ret_l. ss.
+  Qed.
+
+  Lemma interp_thread_nonpreemtive_trigger_yield R tid (ktr : ktree Es () R) :
+    interp_thread_nonpreemtive (tid, x <- trigger (inl1 (inr1 Yield));; ktr x) =
+      Ret (inl (ktr tt)).
+  Proof. rewrite bind_trigger. apply interp_thread_nonpreemtive_vis_yield. Qed.
 
 End SCHEDULE.
